Tests/BimodalTest.lean
@@ -7,6 +7,7 @@ Authors: Benjamin Brast-McKie
 import BimodalTest.Syntax.FormulaTest
 import BimodalTest.Syntax.ContextTest
 import BimodalTest.Syntax.FormulaPropertyTest
+import BimodalTest.Syntax.LanguageDerivationTest
 import BimodalTest.ProofSystem.AxiomsTest
 import BimodalTest.ProofSystem.DerivationTest
 import BimodalTest.ProofSystem.DerivationPropertyTest
